\documentclass[a4paper,11pt, hidelinks]{article}

\usepackage{listings}
\usepackage{lmodern}
\usepackage{amsmath,amssymb,amsthm,textcomp}
\usepackage[utf8]{inputenc}  
\usepackage[T1]{fontenc}  
\usepackage{graphicx}
\usepackage{float}
\usepackage{enumitem}
\usepackage{bbm}
\usepackage{caption}
\usepackage{cancel}
\usepackage{bigints}
\usepackage[colorlinks = true,citecolor = blue, linkcolor = blue,
            urlcolor  = blue,]{hyperref}
\graphicspath{ {images/} }
\usepackage{xcolor}
\usepackage{geometry}
\geometry{total={210mm,297mm},
left=15mm,right=15mm,%
bindingoffset=0mm, top=5mm,bottom=20mm}

\usepackage{etoolbox}
\makeatletter
\preto{\@verbatim}{\topsep=0pt \partopsep=3pt }
\makeatother

\linespread{1}

\newcommand{\linia}{\rule{\linewidth}{0.5pt}}


% my own titles
\makeatletter
\renewcommand{\maketitle}{
\begin{center}
\vspace{2ex}
{\huge \textsc{\@title}}
\vspace{1ex}
\\
\linia\\
\@author 
\vspace{4ex}
\end{center}
}
\makeatother
%%%

% custom footers and headers
\usepackage{fancyhdr}
\pagestyle{fancy}
\lhead{}
\chead{}
\rhead{}

\cfoot{}
\rfoot{Page \thepage}
\renewcommand{\headrulewidth}{0pt}
\renewcommand{\footrulewidth}{0pt}
%
\DeclareMathOperator*{\argmax}{arg\,max}
\DeclareMathOperator*{\argmin}{arg\,min}
\DeclareMathOperator*{\var}{var}
\DeclareMathOperator*{\cov}{cov}

%%%----------%%%----------%%%----------%%%----------%%%

\begin{document}

\title{HW4}

\author{Gabriel ROMON}



\maketitle
{}
\section*{Problem 14.4}
Let us first state some context regarding Hidden Markov Models by following the exposition given in \cite{book:54642}. Given two measurable spaces $(X,\mathcal X)$ and $(Y,\mathcal Y)$, $Q$ a Markov kernel on $(X,\mathcal X)$ and $G$ a Markov kernel from $(X,\mathcal X)$ to $(Y,\mathcal Y)$ we define the following transition kernel on the product space: $$T((x,y),C) = \int 1_C(x,y) G(x',dy')Q(x,dx')$$ Together with the initial distribution $\nu \otimes G$, this defines a Markov chain $(X_k,Y_k)_{k\geq 0}$.\newline
For the case considered in the problem, $(X,\mathcal X)=(\{1,\ldots,\kappa\}, \mathcal P(\{1,\ldots,\kappa\}))$, $(Y,\mathcal Y) = (\mathbb R, \mathcal B(\mathbb R))$ and the model is \textit{fully dominated}, meaning that both kernels have densities. Indeed, $\forall x\in X, Q(x,\cdot) \ll N_X$ where $N_X$ denotes the counting measure on $X$, with density $x'\mapsto \mathbb P_{xx'}$. In addition, $\forall x\in X, G(x,\cdot)\ll \lambda$ with density $y\mapsto f(y|x)$. \newline It follows that the transition kernel $T((x,y),\cdot)$ has density $(x',y')\mapsto t((x,y),(x',y'))=p(x,x')f(y'|x')$.\newline
By a standard result on Markov chains, the joint distribution of $(X_0,Y_0,\ldots, Y_t,Y_t)$ is given by the equality $$\begin{aligned}E(g(X_0,Y_0,\ldots, Y_t,Y_t)) 
&= \int g(x_0,y_0,\ldots,x_t,y_t) \prod_{j=0}^{t-1} T((x_{j},y_{j}),d(x_{j+1},y_{j+1})) \;\nu \otimes G(d(x_0,y_0))\\
&= \int \int \int g(x_0,y_0,\ldots,x_t,y_t) \prod_{j=0}^{t-1} \mathbb P_{x_{j} x_{j+1}} \prod_{j=0}^t f(y_j|x_j) d\lambda^{\otimes t+1}(y_{0:t}) dN_X^{\otimes t}(x_{1:t}) d\nu(x_0)
 \end{aligned}$$
for every bounded measurable function $g$. Consequently, the joint distribution of $(X_1,Y_1,\ldots, Y_t,Y_t)$ is given by 
$$\hspace{-1cm}E(g(X_1,Y_1,\ldots, X_t,Y_t)) = \int \int g(x_1,y_1,\ldots,x_t,y_t) \prod_{j=1}^{t-1}\mathbb P_{x_{j} x_{j+1}} \prod_{j=1}^{t}f(y_j|x_j) p(x_1)d\lambda^{\otimes t}(y_{1:t}) dN_X^{\otimes t}(x_{1:t})$$
where $p(x_1) = \int \int \mathbb P_{x_0 x_1} f(y_0|x_0)d\lambda(y_0)d\nu(x_0)=\int \mathbb P_{x_0 x_1} d\nu(x_0)$.\newline
This implies that the joint density of $(X_1,Y_1,\ldots, Y_t,Y_t)$ with respect to the measure $\lambda^{\otimes t} \otimes N_X^{\otimes t}$ is $$(x_1,y_1,\ldots, x_t,y_t) \mapsto \prod_{j=1}^{t-1}\mathbb P_{x_{j} x_{j+1}} \prod_{j=1}^{t}f(y_j|x_j) p(x_1)$$
We will use this result repeatedly in the problem.

\begin{enumerate}[label=(\alph*)]
	\item We are asked to compute the conditional densities of $X_1,\ldots,X_t$ given $Y_{1:t}=y_{1:t}$ and $X_1,\ldots,X_t$ given $Y_{1:t-1}=y_{1:t-1}$. It suffices to compute the ratio of the joint density and the relevant marginal density.
	$$\begin{aligned}
		p(x_{1:t}|y_{1:t}) &= \frac{\prod_{j=1}^{t-1}\mathbb P_{x_{j} x_{j+1}} \prod_{j=1}^{t}f(y_j|x_j) p(x_1)}{\int \prod_{j=1}^{t-1}\mathbb P_{x_{j} x_{j+1}} \prod_{j=1}^{t}f(y_j|x_j) p(x_1) dN_X^{\otimes t}(x_{1:t})}\\
		&= \begin{aligned}[t]&\frac{\prod_{j=1}^{t-1}\mathbb P_{x_{j} x_{j+1}} \prod_{j=1}^{t}f(y_j|x_j) p(x_1)}{\mathbin{\textcolor{red}{\prod_{j=1}^{t-1}\mathbb P_{x_{j} x_{j+1}} \prod_{j=1}^{t-1}f(y_j|x_j) p(x_1)}}}
		   \frac{\mathbin{\textcolor{red}{\prod_{j=1}^{t-1}\mathbb P_{x_{j} x_{j+1}} \prod_{j=1}^{t-1}f(y_j|x_j) p(x_1)}}}{\mathbin{\textcolor{blue}{\int \prod_{j=1}^{t-1}\mathbb P_{x_{j} x_{j+1}} \prod_{j=1}^{t-1}f(y_j|x_j) p(x_1) dN_X^{\otimes t}(x_{1:t})}}}\\ 
		   \times &\frac{1}{\frac{\int \prod_{j=1}^{t-1}\mathbb P_{x_{j} x_{j+1}} \prod_{j=1}^{t}f(y_j|x_j) p(x_1) dN_X^{\otimes t}(x_{1:t})}{\mathbin{\textcolor{blue}{\int \prod_{j=1}^{t-1}\mathbb P_{x_{j} x_{j+1}} \prod_{j=1}^{t-1}f(y_j|x_j) p(x_1) dN_X^{\otimes t}(x_{1:t})}}}} \end{aligned}\\
		&= f(y_t|x_t) p(x_{1:t}|y_{1:t-1})\frac{1}{p(y_t|y_{1:t-1})}
	\end{aligned} $$
	The red term is the joint density of $(X_{1:t},Y_{1:t-1})$ obtained by marginalizing with respect to $Y_t$, where we used $\int f(y_t|x_t) d\lambda(y_t)= 1$. The blue term is the joint density of $Y_{1:t-1}$ obtained by marginalizing with respect to $(X_{1:t}, Y_t)$.
	$$\begin{aligned}
		p(x_{1:t}|y_{1:t-1}) &= \frac{\prod_{j=1}^{t-1}\mathbb P_{x_{j} x_{j+1}} \prod_{j=1}^{t-1}f(y_j|x_j) p(x_1)}{\int \prod_{j=1}^{t-1}\mathbb P_{x_{j} x_{j+1}} \prod_{j=1}^{t-1}f(y_j|x_j) p(x_1) dN_X^{\otimes t}(x_{1:t})}\\
		&= \mathbb P_{x_{t-1} x_t} \frac{\prod_{j=1}^{t-2}\mathbb P_{x_{j} x_{j+1}} \prod_{j=1}^{t-1}f(y_j|x_j) p(x_1)}{\int \prod_{j=1}^{t-1}\mathbb P_{x_{j} x_{j+1}} \prod_{j=1}^{t-1}f(y_j|x_j) p(x_1) dN_X^{\otimes t}(x_{1:t})}\\
		&= \mathbb P_{x_{t-1} x_t} \frac{p(x_{1:t-1}, y_{1:t-1})}{p(y_{1:t-1})} = \mathbb P_{x_{t-1}x_t}p(x_{1:t-1}|y_{1:t-1})
	\end{aligned} $$

	\item Combining the first actualization equation with the second yields $$p(x_{1:t}|y_{1:t}) = \frac{f(y_t|x_t) \mathbb P_{x_{t-1}x_t}}{p(y_t|y_{1:t-1})}p(x_{1:t-1}|y_{1:t-1})$$
	To compute the filtering density, one needs to get a hold of $p(x_{1:t-1}|y_{1:t-1})$ and $p(y_t|y_{1:t-1})$. The second quantity is linked to the first one in the following way: 
	$$\begin{aligned}
		p(y_t|y_{1:t-1}) &= \frac{\int \prod_{j=1}^{t-1}\mathbb P_{x_{j} x_{j+1}} \prod_{j=1}^{t}f(y_j|x_j) p(x_1) dN_X^{\otimes t}(x_{1:t})}{\int \prod_{j=1}^{t-1}\mathbb P_{x_{j} x_{j+1}} \prod_{j=1}^{t-1}f(y_j|x_j) p(x_1) dN_X^{\otimes t}(x_{1:t})}\\
		&= \int \mathbb P_{x_{t-1} x_t} f(y_t|x_t) \frac{\prod_{j=1}^{t-2}\mathbb P_{x_{j} x_{j+1}} \prod_{j=1}^{t-1}f(y_j|x_j) p(x_1) }{\int \prod_{j=1}^{t-1}\mathbb P_{x_{j} x_{j+1}} \prod_{j=1}^{t-1}f(y_j|x_j) p(x_1) dN_X^{\otimes t}(x_{1:t})} dN_X^{\otimes t}(x_{1:t}) \\
		&= \int \mathbb P_{x_{t-1} x_t} f(y_t|x_t) p(x_{1:t-1}|y_{1:t-1}) dN_X^{\otimes t}(x_{1:t})\\
		&= \sum_{x_1,\ldots,x_t\in X^t} \mathbb P_{x_{t-1} x_t} f(y_t|x_t) p(x_{1:t-1}|y_{1:t-1})
	\end{aligned}$$
	As a result, computing $p(y_t|y_{1:t-1})$ has the same complexity as computing $p(x_{1:t}|y_{1:t})$.

	\item From the actualization equations we already know $p(x_{1:t}|y_{1:t-1})$. $p(x_{t}|y_{1:t-1})$ can then be computed by a simple marginalization:
	$$\begin{aligned}
		p(x_{t}|y_{1:t-1}) &= \int p(x_{t}|y_{1:t-1}) dN_X^{\otimes t-1}(x_{1:t-1}) = \int \mathbb P_{x_{t-1}x_t}p(x_{1:t-1}|y_{1:t-1}) dN_X^{\otimes t-1}(x_{1:t-1})\\
		&= \sum_{x_{1:t-1}\in X^{t-1}} \mathbb P_{x_{t-1}x_t}p(x_{1:t-1}|y_{1:t-1})
	\end{aligned}$$
\end{enumerate}

\section*{Problem 14.5}
\begin{enumerate}[label=(\alph*)]
	\item $\bullet$ Computing $\alpha_1(i)$ boils down to finding the joint density of $(X_1,Y_1)$. Marginalizing like before, 
	$$\begin{aligned}p(y_1,x_1) &= p(x_1)f(y_1|x_1) \int \int \prod_{j=1}^{t-1}\mathbb P_{x_{j} x_{j+1}} \underbrace{\prod_{j=2}^{t}f(y_j|x_j)d\lambda^{\otimes t-1}(y_{2:t})}_{=1} dN_X^{\otimes t-1}(x_{2:t}) \\
	&= p(x_1)f(y_1|x_1) \int \ldots \underbrace{\int \mathbb P_{x_{t-1} x_{t}} dN_X(x_t)}_{=1} \mathbb P_{x_{t-2} x_{t-1}}dN_X(x_{t-1}) \ldots dN_X(x_{2})\\
	&= p(x_1)f(y_1|x_1)
	\end{aligned}
	$$
	Hence $\alpha_1(i) = p(y_1,i)=p(i)f(y_1|i)=\pi_i f(y_1|X_1 =i)$ where the last equality enforces notations used in the statement of the problem.
	\newline
	\newline
	$\bullet$ The recursion for $\alpha_{t+1}(j)$ follows from computing the joint density of $(X_{t+1}, Y_{1:t+1})$:
	$$\begin{aligned}
		p(y_{1:t+1}, x_{t+1}) &= f(y_{t+1}|x_{t+1})\int \prod_{j=1}^{t}\mathbb P_{x_{j} x_{j+1}} \prod_{j=1}^{t}f(y_j|x_j)p(x_1) dN_X^{\otimes t}(x_{1:t}) \\
		&= f(y_{t+1}|x_{t+1}) \int \mathbb P_{x_{t} x_{t+1}} \int \prod_{j=1}^{t-1}\mathbb P_{x_{j} x_{j+1}} \prod_{j=1}^{t}f(y_j|x_j)p(x_1) dN_X^{\otimes t-1}(x_{1:t-1}) dN_X(x_t)\\
		&= f(y_{t+1}|x_{t+1}) \int \mathbb P_{x_{t} x_{t+1}} p(y_{1:t}, x_{t}) dN_X(x_t)\\
		&= f(y_{t+1}|x_{t+1}) \sum_{x_t\in X} \mathbb P_{x_{t} x_{t+1}} \alpha_t(x_t)
	\end{aligned}$$
	Hence $$\alpha_{t+1}(j) = f(y_{t+1}|j) \sum_{x_t\in X} \mathbb P_{x_{t}\;j} \alpha_t(x_t) = f(y_{t+1}|X_{t+1} = j) \sum_{i=1}^\kappa \mathbb P_{ij} \;\alpha_t(i)$$ where the last equality enforces notations used in the statement of the problem.
	\newline
	\newline
	$\bullet$ \textbf{There is a mistake in the statement of the problem (2nd edition of the book)}.\newline $\beta_t(i)$ should be defined as $p(y_{t+1:T}|x_t=i)$ (the conditioning sign is missing). Computing the ratio between the joint and marginal densities yields 
	$$\begin{aligned}
		p(y_{t+1:T}|x_t) &= \frac{\int \prod_{j=1}^{T-1}\mathbb P_{x_{j} x_{j+1}} \prod_{j=1}^{T}f(y_j|x_j)p(x_1) dN_X^{\otimes T-1}(x_{1:T\setminus \{t\}}) d\lambda^{\otimes t}(y_{1:t})}{\int \prod_{j=1}^{t-1}\mathbb P_{x_{j} x_{j+1}} \prod_{j=1}^{t}f(y_j|x_j)p(x_1) dN_X^{\otimes t-1}(x_{1:t-1}) d\lambda^{\otimes t}(y_{1:t})}\\
		&= \frac{\int \prod_{j=1}^{T-1}\mathbb P_{x_{j} x_{j+1}} \prod_{j=t+1}^{T}f(y_j|x_j)p(x_1) dN_X^{\otimes T-1}(x_{1:T\setminus \{t\}}) }{\int \prod_{j=1}^{t-1}\mathbb P_{x_{j} x_{j+1}}p(x_1) dN_X^{\otimes t-1}(x_{1:t-1})}\\
		&= \frac{\int \prod_{j=1}^{T-1}\mathbb P_{x_{j} x_{j+1}} \prod_{j=t+1}^{T}f(y_j|x_j)p(x_1) dN_X^{\otimes T-1}(x_{1:T\setminus \{t\}}) }{\int \prod_{j=1}^{t-1}\mathbb P_{x_{j} x_{j+1}}p(x_1) dN_X^{\otimes t-1}(x_{1:t-1})}\\
		&= \frac{\int \prod_{j=1}^{t-1}\mathbb P_{x_{j} x_{j+1}}p(x_1) dN_X^{\otimes t-1}(x_{1:t-1}) \cdot \int \prod_{j=t}^{T-1}\mathbb P_{x_{j} x_{j+1}} \prod_{j=t+1}^{T}f(y_j|x_j) dN_X^{\otimes T-t}(x_{t+1:T}) }{\int \prod_{j=1}^{t-1}\mathbb P_{x_{j} x_{j+1}} p(x_1)dN_X^{\otimes t-1}(x_{1:t-1})}\\
		&= \mathbin{\textcolor{blue}{\int \prod_{j=t}^{T-1}\mathbb P_{x_{j} x_{j+1}} \prod_{j=t+1}^{T}f(y_j|x_j) dN_X^{\otimes T-t}(x_{t+1:T})}} \\
		&= \int \mathbb P_{x_t x_{t+1}}f(y_{t+1}|x_{t+1}) \mathbin{\textcolor{red}{\int \prod_{j=t+1}^{T-1}\mathbb P_{x_{j} x_{j+1}} \prod_{j=t+2}^{T}f(y_j|x_j) dN_X^{\otimes T-t-1}(x_{t+2:T})}} dN_X(x_{t+1})
	\end{aligned} $$
	The red term is identical to the blue one, except that $t$ is replaced by $t+1$. Since the blue term is $p(y_{t+1:T}|x_t)$, the red one is $p(y_{t+2:T}|x_{t+1})$, hence 
	$$\begin{aligned}
	p(y_{t+1:T}|x_t) &= \int \mathbb P_{x_t x_{t+1}}f(y_{t+1}|x_{t+1}) p(y_{t+2:T}|x_{t+1}) dN_X(x_{t+1}) \\
	&= \sum_{x_{t+1}\in X} \mathbb P_{x_t x_{t+1}}f(y_{t+1}|x_{t+1}) p(y_{t+2:T}|x_{t+1})
	\end{aligned}
	$$
	Consequently, $$\begin{aligned}
	\beta_t(i) &= \sum_{x_{t+1}\in X} \mathbb P_{i\;x_{t+1}}f(y_{t+1}|x_{t+1}) \beta_{t+1}(x_{t+1})
	= \sum_{j=1}^{\kappa} \mathbb P_{ij}f(y_{t+1}|j) \beta_{t+1}(j)\\
	&= \sum_{j=1}^{\kappa} \mathbb P_{ij} \;f(y_{t+1}|X_{t+1} = j) \beta_{t+1}(j)
	\end{aligned}
	$$
	where the last equality enforces notations used in the statement of the problem.
	\newline
	\newline
	$\bullet$ Marginalizing yields $$\begin{aligned}
		p(x_t, y_{1:T}) &= \int \prod_{j=1}^{T-1}\mathbb P_{x_{j} x_{j+1}} \prod_{j=1}^{T}f(y_j|x_j) p(x_1) dN_X^{\otimes T-1}(x_{1:T\setminus \{t\}}) \\
		&= \begin{aligned}[t]&\int \prod_{j=1}^{t-1}\mathbb P_{x_{j} x_{j+1}}\prod_{j=1}^{t}f(y_j|x_j) p(x_1) dN_X^{\otimes t-1}(x_{1:t-1})\\ &\times \int \prod_{j=t}^{T-1}\mathbb P_{x_{j} x_{j+1}} \prod_{j=t+1}^{T}f(y_j|x_j) dN_X^{\otimes T-t}(x_{t+1:T}) \end{aligned}\\
		&= p(x_t, y_{1:t})\; p(y_{t+1:T}|x_t)
	\end{aligned} $$
	The last equality follows from identification of each of the integrals: the first one is an obvious marginalization that yields $p(x_t, y_{1:t})$ and the second is the blue term computed a few moments ago, and we proved it is equal to $p(y_{t+1:T}|x_t)$.
	Besides, $$
		p(y_{1:T}) = \int p(x_t, y_{1:T}) dN_X(x_t) = \int p(x_t, y_{1:t})\; p(y_{t+1:T}|x_t) dN_X(x_t)$$
	Hence $$p(x_t| y_{1:T}) = \frac{p(x_t, y_{1:t})\; p(y_{t+1:T}|x_t)}{\int p(x_t, y_{1:t})\; p(y_{t+1:T}|x_t) dN_X(x_t)} = \frac{\alpha_t(x_t)\beta_t(x_t)}{\sum_{x_t\in X} \alpha_t(x_t)\beta_t(x_t) }$$
	and finally $$ \gamma_t(i) = \frac{\alpha_t(i)\beta_t(i)}{\sum_{j=1}^\kappa \alpha_t(j)\beta_t(j)}$$

	\item Let us assume first that all the $\alpha_t(i)$ and $\beta_t(i)$ have already been computed and stored in memory. We begin with a naive evaluation: for fixed $t$ and $i$, computing $\gamma_t(i)$ requires computing $\sum_{j=1}^\kappa \alpha_t(j)\beta_t(j)$, which takes $O(\kappa)$, hence a global time complexity of $O(T\kappa^2)$.\newline However, this is clearly inefficient since $\sum_{j=1}^\kappa \alpha_t(j)\beta_t(j)$ may be only evaluated once and stored in memory. For a given $t$, we compute all the $\alpha_t(i)\beta_t(i)$, then the sum $\sum_{j=1}^\kappa \alpha_t(j)\beta_t(j)$ and finally the ratios, yielding all the $\gamma_t(i)$ with a time complexity of $O(\kappa + \kappa + \kappa) = O(\kappa)$, hence a global complexity of $O(T\kappa)$.\newline
	\newline
	For a more realistic evaluation we assume that the $\alpha_t(i)$ and $\beta_t(i)$ are not known and need to be computed beforehand. Since recursive programming results in a lot of repeated computations, it is inefficient and we turn to dynamic programming instead. Computing all the $\alpha_1(i)$ takes $O(\kappa)$. By storing $\alpha_{t}$ in memory, evaluating $\alpha_{t+1}(j)$ for each $j$ is $O(\kappa)$, hence computing $\alpha_{t+1}$ takes $O(\kappa^2)$, yielding a total time complexity of $O(\kappa) + \sum_{t=2}^T O(\kappa^2) = O(T\kappa^2)$ to compute $\alpha$. In a similar fashion, the evaluation of $\beta$ requires $O(T\kappa^2)$ in time. Finally, computing $\gamma$ from scratch has complexity $O(T\kappa^2) + O(T\kappa^2) + O(T\kappa) = O(T\kappa^2)$.

	\item Let us compute the joint density of $(X_t,X_{t+1},Y_{1:T})$ by marginalizing: 
	$$\begin{aligned}
		p(x_t,x_{t+1},y_{1:T}) &= \int \prod_{j=1}^{T-1}\mathbb P_{x_{j} x_{j+1}} \prod_{j=1}^{T}f(y_j|x_j)p(x_1) dN_X^{\otimes T-2}(x_{1:T\setminus \{t,t+1\}})\\
		&= \begin{aligned}[t]
			&\int \prod_{j=1}^{t-1}\mathbb P_{x_{j} x_{j+1}} \prod_{j=1}^{t}f(y_j|x_j)p(x_1) dN_X^{\otimes t-1}(x_{1:t-1})\\
			&\times \mathbb P_{x_t x_{t+1}} f(y_{t+1}|x_{t+1})\\
			&\times \int \prod_{j=t+1}^{T-1}\mathbb P_{x_{j} x_{j+1}} \prod_{j=t+2}^{T}f(y_j|x_j) dN_X^{\otimes T-t-1}(x_{t+2:T})
		\end{aligned}\\
		&= p(y_{1:t},x_t) \mathbb P_{x_t x_{t+1}} f(y_{t+1}|x_{t+1}) p(y_{t+2:T}|x_{t+1})
	\end{aligned}$$
	In the second equality, the first integral is a straight marginalization that yields $p(y_{1:t},x_t)$ and the last integral is the red term computed in (a), which was shown to be $p(y_{t+2:T}|x_{t+1})$. Therefore, 
	$$p(x_t,x_{t+1}|y_{1:T}) = \frac{p(y_{1:t},x_t) \mathbb P_{x_t x_{t+1}} f(y_{t+1}|x_{t+1}) p(y_{t+2:T}|x_{t+1})}{\int p(y_{1:t},x_t) \mathbb P_{x_t x_{t+1}} f(y_{t+1}|x_{t+1}) p(y_{t+2:T}|x_{t+1})dN_X^{\otimes 2}(x_{t:t+1})}$$
	Hence 
	$$\begin{aligned}\xi_t(i,j) &= p(i,j|y_{1:T}) = \frac{p(y_{1:t},i) \mathbb P_{ij} f(y_{t+1}|j) p(y_{t+2:T}|j)}{\sum_{i=1}^\kappa \sum_{j=1}^\kappa p(y_{1:t},i) \mathbb P_{ij} f(y_{t+1}|j) p(y_{t+2:T}|j)}\\
	&= \frac{\alpha_t(i) \mathbb P_{ij} f(y_{t+1}|j) \beta_{t+1}(j)}{\sum_{i=1}^\kappa \sum_{j=1}^\kappa \alpha_t(i) \mathbb P_{ij} f(y_{t+1}|j) \beta_{t+1}(j)}
	\end{aligned}$$
	Computing $\alpha$ and $\beta$ has complexity $O(T\kappa^2)$ as shown before. For a fixed $t$, we compute all the numerators in $O(\kappa^2)$, then evaluate the sum $\sum_{i=1}^\kappa \sum_{j=1}^\kappa \alpha_t(i) \mathbb P_{ij} f(y_{t+1}|j) \beta_{t+1}(j)$ in $O(\kappa^2)$ and finally compute all the ratios also in $O(\kappa^2)$, yielding a total time complexity of $O(T(\kappa^2+\kappa^2+\kappa^2)) = O(T\kappa^2)$.

	\item Let $\alpha_t'(i) = \frac{\alpha_t(i)}{c_t}$ and note that $$\frac{\alpha_t'(i)\beta_t(i)}{\sum_{j=1}^\kappa \alpha_t'(j)\beta_t(j)} = \frac{\frac{\alpha_t(i)}{c_t}\beta_t(i)}{\sum_{j=1}^\kappa \frac{\alpha_t(j)}{c_t}\beta_t(j)}=\frac{\alpha_t(i)\beta_t(i)}{\sum_{j=1}^\kappa \alpha_t(j)\beta_t(j)} = \gamma_t(i) $$
	Hence the equalities for $\gamma$ are preserved.
\end{enumerate}

\section*{Problem 14.6}
\begin{enumerate}[label=(\alph*)]
	\item For $s\geq 3$, $$\begin{aligned}
		p(x_s,x_{s-1},y_{1:t}) &= \int \prod_{j=1}^{t-1}\mathbb P_{x_{j} x_{j+1}} \prod_{j=1}^{t}f(y_j|x_j)p(x_1) dN_X^{\otimes t-2}(x_{1:t\setminus \{s-1,s\}}) \\
		&= \begin{aligned}[t]&\int \prod_{j=1}^{s-2}\mathbb P_{x_{j} x_{j+1}} \prod_{j=1}^{s-1}f(y_j|x_j)p(x_1) dN_X^{\otimes s-2}(x_{1:s-2}) \\
							& \times \mathbb P_{x_{s-1} x_s} f(y_s|x_s)\\
							& \times \int \prod_{j=s}^{t-1}\mathbb P_{x_{j} x_{j+1}} \prod_{j=s+1}^{t}f(y_j|x_j)dN_X^{\otimes t-s}(x_{s+1:t}) 
			\end{aligned}\\
		&= \begin{aligned}[t]& p(x_{s-1},y_{1:s-1}) \\
							& \times \mathbb P_{x_{s-1} x_s} f(y_s|x_s)\\
							& \times \int \prod_{j=s}^{t-1}\mathbb P_{x_{j} x_{j+1}} \prod_{j=s+1}^{t}f(y_j|x_j)dN_X^{\otimes t-s}(x_{s+1:t}) \quad \quad \quad (*)
			\end{aligned} 
	\end{aligned}$$
	Since $p(x_{s-1},y_{1:s-1})$ does not depend on $x_s$, it vanishes when computing the conditional density: $$p(x_s|x_{s-1},y_{1:t}) = \frac{\mathbb P_{x_{s-1} x_s} f(y_s|x_s) \int \prod_{j=s}^{t-1}\mathbb P_{x_{j} x_{j+1}} \prod_{j=s+1}^{t}f(y_j|x_j)dN_X^{\otimes t-s}(x_{s+1:t})}{\int \mathbb P_{x_{s-1} x_s} f(y_s|x_s) \int \prod_{j=s}^{t-1}\mathbb P_{x_{j} x_{j+1}} \prod_{j=s+1}^{t}f(y_j|x_j)dN_X^{\otimes t-s}(x_{s+1:t}) dN_X(x_s)}$$
	A similar computation yields 
	$$\begin{aligned}
		p(x_s,x_{s-1},y_{s:t}) &= \begin{aligned}[t]& p(x_{s-1}) \\
							& \times \mathbb P_{x_{s-1} x_s} f(y_s|x_s)\\
							& \times \int \prod_{j=s}^{t-1}\mathbb P_{x_{j} x_{j+1}} \prod_{j=s+1}^{t}f(y_j|x_j)dN_X^{\otimes t-s}(x_{s+1:t}) 
			\end{aligned}
	\end{aligned}$$
	$p(x_{s-1})$ vanishes and we get $$\hspace{-0.8cm}p(x_s|x_{s-1},y_{s:t}) = \frac{\mathbb P_{x_{s-1} x_s} f(y_s|x_s) \int \prod_{j=s}^{t-1}\mathbb P_{x_{j} x_{j+1}} \prod_{j=s+1}^{t}f(y_j|x_j)dN_X^{\otimes t-s}(x_{s+1:t})}{\int \mathbb P_{x_{s-1} x_s} f(y_s|x_s) \int \prod_{j=s}^{t-1}\mathbb P_{x_{j} x_{j+1}} \prod_{j=s+1}^{t}f(y_j|x_j)dN_X^{\otimes t-s}(x_{s+1:t}) dN_X(x_s)} = p(x_s|x_{s-1},y_{1:t})$$
	For $s=2$ the equality is proved in a similar fashion.

	\item 
	$\bullet$ Note that $$\begin{aligned}p(x_t,x_{t-1},y_{1:t}) &= \mathbb P_{x_{t-1} x_t} f(y_t|x_t) \int \prod_{j=1}^{t-2}\mathbb P_{x_{j} x_{j+1}} \prod_{j=1}^{t-1}f(y_j|x_j)p(x_1) dN_X^{\otimes t-2}(x_{1:t-2})\\ &=  \mathbb P_{x_{t-1} x_t} f(y_t|x_t) p(x_{t-1},y_{1:t-1})\end{aligned}$$
	Hence $\displaystyle p(x_t|x_{t-1},y_{1:t}) = \mathbb P_{x_{t-1} x_t} f(y_t|x_t) \frac{p(x_{t-1},y_{1:t-1})}{p(x_{t-1},y_{1:t})}$ and we define an unnormalized version of this conditional density as $p_t^\star(x_t|x_{t-1},y_{1:t}) := \mathbb P_{x_{t-1} x_t} f(y_t|x_t)$.
	\newline
	\newline
	$\bullet$ Let $2\leq s \leq t-1$. From equation $(*)$ in (a) we have 
	$$\begin{aligned} p(x_s,x_{s-1},y_{1:t}) &= p(x_{s-1},y_{1:s-1})\mathbb P_{x_{s-1} x_s} f(y_s|x_s)\int \prod_{j=s}^{t-1}\mathbb P_{x_{j} x_{j+1}} \prod_{j=s+1}^{t}f(y_j|x_j)dN_X^{\otimes t-s}(x_{s+1:t}) \\
	&= p(x_{s-1},y_{1:s-1})\mathbb P_{x_{s-1} x_s} f(y_s|x_s) \int \frac{p(x_{s+1},x_{s},y_{1:t})}{p(x_{s},y_{1:s})} dN_X(x_{s+1})\\
	&= \mathbb P_{x_{s-1} x_s} f(y_s|x_s) \int p(x_{s+1}|x_{s},y_{1:t}) \frac{p(x_{s},y_{1:t})}{p(x_{s},y_{1:s})} dN_X(x_{s+1}) p(x_{s-1},y_{1:s-1})
	\end{aligned}$$
	Hence $$p(x_s|x_{s-1},y_{1:t}) = \mathbb P_{x_{s-1} x_s} f(y_s|x_s) \sum_{x_{s+1}\in X} \left[p(x_{s+1}|x_{s},y_{1:t}) \frac{p(x_{s},y_{1:t})}{p(x_{s},y_{1:s})}\right]  \frac{p(x_{s-1},y_{1:s-1})}{p(x_{s-1},y_{1:t})}$$
	and we let $$p_s^\star(x_s|x_{s-1},y_{1:t}) := \mathbb P_{x_{s-1} x_s} f(y_s|x_s) \sum_{x_{s+1}\in X} \left[p(x_{s+1}|x_{s},y_{1:t}) \frac{p(x_{s},y_{1:t})}{p(x_{s},y_{1:s})}\right]$$
	\newline
	$\bullet$ Note that $$\begin{aligned}
		p(x_1,y_{1:t}) &= p(x_1) f(y_1|x_1) \int \mathbb P_{x_{1} x_{2}} f(y_2|x_2) \prod_{j=2}^{t-1}\mathbb P_{x_{j} x_{j+1}} \prod_{j=3}^{t}f(y_j|x_j)p(x_1) dN_X^{\otimes t-2}(x_{1:t-2})\\
		&= p(x_1) f(y_1|x_1) \int \frac{p(x_2,x_1,y_{1:t})}{p(x_1,y_1)} dN_X(x_2)
	\end{aligned}$$
	where we used $(*)$ in the second equality.\newline
	Hence $\displaystyle p(x_1|y_{1:t}) = p(x_1) f(y_1|x_1) \sum_{x_2\in X} \left[p(x_2|x_1,y_{1:t}) \frac{p(x_1,y_{1:t})}{p(x_1,y_1)}\right] \frac{1}{p(y_{1:t})} \quad \quad (**) \quad $ and we let $$p_1^\star(x_1|y_{1:t}) := p(x_1) f(y_1|x_1) \sum_{x_2\in X} \left[p(x_2|x_1,y_{1:t}) \frac{p(x_1,y_{1:t})}{p(x_1,y_1)}\right]$$
	
	$\bullet$ Putting all these relations together we have the following recursion $$\begin{cases}
		\displaystyle p_t^\star(x_t|x_{t-1},y_{1:t}) = \mathbb P_{x_{t-1} x_t} f(y_t|x_t)\\
		\displaystyle p_s^\star(x_s|x_{s-1},y_{1:t}) = \mathbb P_{x_{s-1} x_s} f(y_s|x_s) \sum_{x_{s+1}\in X} p_{s+1}^\star(x_{s+1}|x_{s},y_{1:t})\quad \quad 2\leq s \leq t-1\\
		\displaystyle p_1^\star(x_1|y_{1:t}) = p(x_1) f(y_1|x_1) \sum_{x_2\in X} p_2^\star(x_2|x_1,y_{1:t})
	\end{cases}$$
	We resort to dynamic programming again. For each $1\leq s\leq t-1$ and each $x_s\in \{1,\ldots,\kappa\}$, we must compute a sum of $\kappa$ terms, hence a global time complexity of $O(t\kappa^2)$.

	\item It is straightforward to prove that $\displaystyle p(x_{1:t}|y_{1:t}) = p(x_1|y_{1:t}) \prod_{s=1}^t p(x_s|x_{s-1},y_{1:t})$.\newline 
	Once the ${p_s}^\star$ have been computed, the normalized versions $p(x_s|x_{s-1},y_{1:t})$ can be retrieved without increasing the computational complexity. Given the factorization of the joint distribution, we can sample from it by sequentially generating $x_1$ from $p(x_1|y_{1:t})$, $x_2$ from $p(x_2|x_{1},y_{1:t})$ and so on. This process takes $O(t\kappa^2)$ in time.

	\item Using the formula for $p(x_{1:t}|y_{1:t})$ proved a bit later in (e), we have for $s\geq 3$ $$p(x_{1:s}|y_{1:s}) = \mathbb P_{x_{s-1} x_s} f(y_s|x_s) p(x_{1:s-1}|y_{1:s-1}) \frac{p(y_{1:s-1})}{p(y_{1:s})}$$
	Hence  $$\begin{aligned}
	\argmax_{x_{1:t}} p(x_{1:t}|y_{1:t}) &= \argmax_{x_t}\left[\mathbin{\textcolor{blue}{\argmax_{x_{1:t-1}} p(x_{1:t}|y_{1:t})}} \right]\\
	&= \argmax_{x_t}\left[\argmax_{x_{1:t-1}}\mathbb P_{x_{t-1} x_t} f(y_t|x_t) p(x_{1:t-1}|y_{1:t-1}) \right]\\
	&= \argmax_{x_t}\left[\argmax_{x_{t-1}}\left( \mathbb P_{x_{t-1} x_t} f(y_t|x_t) \mathbin{\textcolor{blue}{\argmax_{x_{1:t-2}} p(x_{1:t-1}|y_{1:t-1})}} \right)\right]
	\end{aligned}
	$$
	The blue terms show that computing the maximizer is amenable to dynamic programming. One starts by computing $$\argmax_{x_{1}} p(x_{1:2}|y_{1:2}) = \argmax_{x_{1}} \mathbb P_{x_{1} x_2} f(y_1|x_1)p(x_1)$$
	and then recurses all the way up to $\argmax_{x_{1:t}} p(x_{1:t}|y_{1:t})$.

	\item Equation $(**)$ in (b) rewrites further as $$p(x_1|y_{1:t}) =  \frac{p_1^\star(x_1|y_{1:t})}{p(y_{1:t})}$$
	Hence $p(y_{1:t}) = \sum_{x_1\in X} p_1^\star(x_1|y_{1:t})$, which yields a representation of the observed likelihood.\newline \newline
	As an aside, $$\begin{aligned}
	p(x_{1:t}|y_{1:t})  &= \begin{aligned}[t]&\frac{p(x_1) f(y_1|x_1) \sum_{x_2\in X} p_2^\star(x_2|x_1,y_{1:t})}{\sum_{x_1\in X} p_1^\star(x_1|y_{1:t})} \prod_{s=1}^{t-1} \frac{\mathbb P_{x_{s-1} x_s} f(y_s|x_s) \sum_{x_{s+1}\in X} p_{s+1}^\star(x_{s+1}|x_{s},y_{1:t})}{\sum_{x_s\in X} p_s^\star(x_s|x_{s-1},y_{1:t})}\\ &\times \frac{\mathbb P_{x_{t-1} x_t} f(y_t|x_t)}{\sum_{x_t\in X} p_t^\star(x_t|x_{t-1},y_{1:t})}\end{aligned}\\
	&= \frac{\prod_{j=1}^{t-1}\mathbb P_{x_{j} x_{j+1}} \prod_{j=1}^{t}f(y_j|x_j)p(x_1)}{\sum_{x_1\in X} p_1^\star(x_1|y_{1:t})}\\
	&= \frac{\prod_{j=1}^{t-1}\mathbb P_{x_{j} x_{j+1}} \prod_{j=1}^{t}f(y_j|x_j)p(x_1)}{p(y_{1:t})}
	\end{aligned}
	$$
	
	\item As stated in (c), computing the conditional likelihood $p(x_{1:T}|y_{1:T})$ has complexity $O(T\kappa^2)$ in time.
\end{enumerate}

\newpage
\bibliographystyle{unsrt}
\bibliography{bibli}

\end{document}